silveroak-opentitan/aes/Spec/InterleavedCipher.v
@@ -79,9 +79,6 @@ Section Spec.
 
       (* get the key *pairs* *)
       pose proof all_keys_eq as Hall_keys.
-      map_inversion Hall_keys; subst.
-      match goal with H : @eq (list key) _ (_ :: _ ++ [_]) |- _ =>
-                      rename H into Hall_keys end.
 
       cbv [cipher_interleaved cipher_round_interleaved Cipher.cipher].
       rewrite fold_left_to_seq with (default:=initial_key).
@@ -151,4 +148,28 @@ Section Spec.
         reflexivity. }
     Qed.
   End Equivalence.
+
+  (* assume key_expand and all subroutines are the *inverse* operations, and
+     prove equivalent to inverse cipher *)
+  Section InverseEquivalence.
+    Context (Nr : nat) (initial_key : key)
+            (first_key : key) (middle_keys : list key) (last_key : key).
+    Context (all_keys_eq :
+               all_keys key_expand Nr initial_key
+               = first_key :: middle_keys ++ [last_key]).
+
+    Let inverse_cipher :=
+      equivalent_inverse_cipher
+        state key add_round_key sub_bytes shift_rows mix_columns.
+
+    (* Interleaved cipher is equivalent to original cipher *)
+    Lemma inverse_cipher_interleaved_equiv input :
+      cipher_interleaved Nr initial_key input =
+      inverse_cipher first_key last_key middle_keys input.
+    Proof.
+      intros. subst inverse_cipher.
+      erewrite cipher_interleaved_equiv by eassumption.
+      reflexivity.
+    Qed.
+  End InverseEquivalence.
 End Spec.
